Extend the language with `let x = e1 in e2` expressions

Stlc.v
@@ -5,11 +5,58 @@ Require Import Coq.FSets.FMaps.
 Require Import Coq.MSets.MSets.
 Require Import Coq.Structures.Equalities.
 
+Lemma not_None_implies_Some : forall {A : Set} (o : option A),
+  o <> None -> exists x, o = Some x.
+Proof.
+  intros A o H.
+  destruct o.
+  - exists a. reflexivity.
+  - congruence.
+Qed.
+
 Module Var := Nat.
 Definition var : Set := Var.t.
 Module VarSet := MSetAVL.Make Var.
 Module VarSetFacts := MSetFacts.Facts VarSet.
 Module VarSetProps := MSetProperties.Properties VarSet.
+
+Lemma VarSet_For_all_Empty : forall P s,
+  VarSet.Empty s ->
+  VarSet.For_all P s.
+Proof.
+  intros P s H1 x H2.
+  apply VarSetProps.empty_is_empty_1 in H1.
+  rewrite H1 in H2.
+  apply VarSetFacts.empty_iff in H2.
+  inversion H2.
+Qed.
+
+Lemma VarSet_For_all_union_spec : forall P s s',
+  VarSet.For_all P (VarSet.union s s') ->
+  VarSet.For_all P s /\ VarSet.For_all P s'.
+Proof.
+  intros P s s' H.
+  induction s using VarSetProps.set_induction; subst.
+  - apply VarSetProps.empty_is_empty_1 in H0.
+    split.
+    + intros x contra.
+      rewrite H0 in contra.
+      apply VarSetFacts.empty_iff in contra.
+      inversion contra.
+    + intros x H2.
+      specialize (H x).
+      apply VarSetFacts.union_3 with (s:=s) in H2.
+      auto.
+  - split.
+    + intros y H2.
+      specialize (H y).
+      apply VarSetFacts.union_2 with (s':=s') in H2.
+      auto.
+    + intros y H2.
+      unfold VarSet.For_all in H.
+      apply VarSetFacts.union_3 with (s:=s2) in H2.
+      auto.
+Qed.
 
 Inductive type : Set :=
 | tunit : type
@@ -19,14 +66,16 @@ Inductive expr : Set :=
 | eunit : expr
 | evar : var -> expr
 | eabs : var -> type -> expr -> expr
-| eapp : expr -> expr -> expr.
+| eapp : expr -> expr -> expr
+| elet : var -> expr -> expr -> expr.
 
 Fixpoint free_vars (e : expr) : VarSet.t :=
   match e with
   | eunit => VarSet.empty
-  | evar y => VarSet.singleton y
-  | eabs y _ e => VarSet.remove y (free_vars e)
+  | evar x => VarSet.singleton x
+  | eabs x _ e => VarSet.remove x (free_vars e)
   | eapp e1 e2 => VarSet.union (free_vars e1) (free_vars e2)
+  | elet x e1 e2 => VarSet.union (free_vars e1) (VarSet.remove x (free_vars e2))
   end.
 
 (* Type system *)
@@ -52,7 +101,12 @@ Inductive has_type : context -> expr -> type -> Prop :=
 | has_type_app : forall c e1 e2 t1 t2,
     has_type c e1 (tfun t1 t2) ->
     has_type c e2 t1 ->
-    has_type c (eapp e1 e2) t2.
+    has_type c (eapp e1 e2) t2
+
+| has_type_let : forall c x e1 e2 t1 t2,
+    has_type c e1 t1 ->
+    has_type (Context.add x t1 c) e2 t2 ->
+    has_type c (elet x e1 e2) t2.
 
 
 (* Small-step semantics *)
@@ -69,60 +123,168 @@ Fixpoint subst (x : var) (e1 e2 : expr) :=
       (* Assuming y is not free in e1 *)
       (if Var.eqb x y then e else subst x e1 e)
   | eapp e3 e4 => eapp (subst x e1 e3) (subst x e1 e4)
+  | elet y e3 e4 => elet y (subst x e1 e3)
+      (* Assuming y is not free in e1 *)
+      (if Var.eqb x y then e4 else subst x e1 e4)
   end.
 
-Inductive eval : expr -> expr -> Prop :=
-| eval_app1 : forall e1 e2 v1, 
-    eval e1 v1 ->
-    eval (eapp e1 e2) (eapp v1 e2)
+Module Heap := FMapWeakList.Make Var.
+Module HeapFacts := FMapFacts.Facts Heap.
+Module HeapProps := FMapFacts.Properties Heap.
+Definition heap := Heap.t expr.
+Definition heap_empty : heap := Heap.empty expr.
 
-| eval_app2 : forall e2 v1 v2, 
+Inductive eval : heap -> expr -> expr -> Prop :=
+| eval_var : forall h x e,
+    Heap.find x h = Some e->
+    eval h (evar x) e
+
+| eval_app1 : forall h e1 e2 v1, 
+    eval h e1 v1 ->
+    eval h (eapp e1 e2) (eapp v1 e2)
+
+| eval_app2 : forall h e2 v1 v2, 
     value v1 ->
-    eval e2 v2 ->
-    eval (eapp v1 e2) (eapp v1 v2)
+    eval h e2 v2 ->
+    eval h (eapp v1 e2) (eapp v1 v2)
 
-| eval_beta : forall x t e v2,
+| eval_beta : forall h x t e v2,
     value v2 ->
-    eval (eapp (eabs x t e) v2) (subst x v2 e).
+    eval h (eapp (eabs x t e) v2) (subst x v2 e)
 
-Inductive eval_star : expr -> expr -> Prop :=
-| eval_star_refl : forall e,
-    eval_star e e
+| eval_let1 : forall h x e1 e2 e3,
+    eval h e1 e3 ->
+    eval h (elet x e1 e2) (elet x e3 e2)
 
-| eval_star_step : forall e1 e2 e3,
-    eval e1 e2 ->
-    eval_star e2 e3 ->
-    eval_star e1 e3.
+| eval_let2 : forall h x v1 e2,
+    value v1 ->
+    eval h (elet x v1 e2) (subst x v1 e2).
+
+Inductive eval_star : heap -> expr -> expr -> Prop :=
+| eval_star_refl : forall h e,
+    eval_star h e e
+
+| eval_star_step : forall h e1 e2 e3,
+    eval h e1 e2 ->
+    eval_star h e2 e3 ->
+    eval_star h e1 e3.
 
 
 (* Type safety *)
 
+Lemma VarSet_For_all_remove : forall x (h : heap) s e,
+  VarSet.For_all (fun y => Heap.In y h) (VarSet.remove x s) ->
+  VarSet.For_all (fun y => Heap.In y (Heap.add x e h)) s.
+Proof.
+  intros x h s e H1 z H2.
+  destruct (Var.eqb x z) eqn:Heqn.
+  - apply Var.eqb_eq in Heqn; subst.
+    apply HeapFacts.add_in_iff.
+    auto.
+  - apply Var.eqb_neq in Heqn.
+    specialize (H1 z).
+    simpl in H1.
+    apply VarSetFacts.remove_2 with (x:=x) in H2; try assumption.
+    apply HeapFacts.add_in_iff.
+    auto.
+Qed.
+
+Lemma progress0 : forall c e1 t (h : heap),
+  has_type c e1 t ->
+  VarSet.For_all (fun x => Heap.In x h) (free_vars e1) ->
+  value e1 \/ exists e2, eval h e1 e2.
+Proof.
+  intros c e1 t h HAS_TYPE.
+  generalize dependent h.
+  induction HAS_TYPE; intros h HH.
+  - auto using vunit.
+  - right.
+    unfold VarSet.For_all in HH.
+    specialize (HH x (VarSetFacts.singleton_2 eq_refl)).
+    apply HeapFacts.in_find_iff in HH.
+    apply not_None_implies_Some in HH as [e3 HH].
+    exists e3.
+    auto using eval_var.
+  - auto using vabs.
+  - right.
+    simpl in HH.
+    apply VarSet_For_all_union_spec in HH as [H1 H2].
+    specialize (IHHAS_TYPE1 _ H1) as [IH1 | [e3 IH1]]; clear H1.
+    + specialize (IHHAS_TYPE2 _ H2) as [IH2 | [e4 IH2]]; clear H2.
+      * destruct e1; inversion HAS_TYPE1; inversion IH1; subst.
+        exists (subst v e2 e1). auto using eval_beta.
+      * exists (eapp e1 e4). auto using eval_app2.
+    + exists (eapp e3 e2). auto using eval_app1.
+  - right.
+    simpl in HH.
+    apply VarSet_For_all_union_spec in HH as [H1 H2].
+    specialize (IHHAS_TYPE1 h H1) as [IH1 | [e3 IH1]]; clear H1.
+    + apply VarSet_For_all_remove with (e:=e1) in H2.
+      exists (subst x e1 e2). auto using eval_let2.
+    + exists (elet x e3 e2). auto using eval_let1.
+Qed.
+
+Lemma has_type_free_vars_in_context : forall c e t,
+  has_type c e t ->
+  VarSet.For_all (fun x => Context.mem x c = true) (free_vars e).
+Proof.
+  intros c e t H.
+  induction H; simpl.
+  - intros x contra.
+    apply VarSetFacts.empty_iff in contra.
+    inversion contra.
+  - intros y H2.
+    apply Context.mem_1.
+    apply ContextFacts.in_find_iff.
+    apply VarSet.singleton_spec in H2.
+    subst.
+    rewrite H.
+    discriminate.
+  - intros y H2.
+    unfold VarSet.For_all in *.
+    apply VarSet.remove_spec in H2 as [H2 H3].
+    specialize (IHhas_type y H2).
+    rewrite ContextFacts.add_neq_b in IHhas_type; auto.
+  - intros x H2.
+    apply VarSet.union_spec in H2 as [H2 | H2]; auto.
+  - intros y H1.
+    apply VarSet.union_spec in H1 as [H1 | H1].
+    + auto.
+    + apply VarSet.remove_spec in H1 as [H1 H2].
+      apply IHhas_type2 in H1.
+      apply not_eq_sym in H2.
+      rewrite ContextFacts.add_neq_b in H1; assumption.
+Qed.
+
+Lemma has_type_empty_context_free_vars : forall e t,
+  has_type context_empty e t ->
+  VarSet.Empty (free_vars e).
+Proof.
+  intros e t H.
+  apply has_type_free_vars_in_context in H.
+  induction (free_vars e) using VarSetProps.set_induction.
+  - assumption.
+  - rename t0_1 into s.
+    rename t0_2 into s'.
+    apply VarSetProps.Add_Equal in H1.
+    unfold VarSet.For_all in *.
+    specialize (H x).
+    rewrite H1 in H.
+    specialize (H (VarSetFacts.add_1 s eq_refl)).
+    rewrite ContextFacts.empty_a in H.
+    discriminate.
+Qed.
+
 Theorem progress : forall e1 t,
   has_type context_empty e1 t ->
-  value e1 \/ exists e2, eval e1 e2.
+  value e1 \/ exists e2, eval heap_empty e1 e2.
 Proof.
   intros e1 t HAS_TYPE.
-  remember context_empty as c eqn:CONTEXT.
-  induction HAS_TYPE; subst c.
-  - auto using value.
-  - rewrite ContextFacts.empty_o in H. inversion H.
-  - auto using value.
-  - right.
-    rename IHHAS_TYPE2 into IH2; specialize (IH2 eq_refl).
-    rename IHHAS_TYPE1 into IH1; specialize (IH1 eq_refl).
-    destruct IH1 as [IH1 | IH1];
-      destruct IH2 as [IH2 | IH2].
-    + inversion IH1; subst.
-      * inversion HAS_TYPE1.
-      * exists (subst x e2 e); auto using eval_beta.
-    + inversion IH1; subst.
-      * inversion HAS_TYPE1.
-      * destruct IH2 as [e3 IH2].
-        exists (eapp (eabs x t e) e3); auto using eval_app2.
-    + destruct IH1 as [e1' IH1].
-      exists (eapp e1' e2); auto using eval_app1.
-    + destruct IH1 as [e1' IH1].
-      exists (eapp e1' e2); auto using eval_app1.
+  apply progress0 with (c:=context_empty) (t:=t).
+  - assumption.
+  - apply has_type_empty_context_free_vars in HAS_TYPE.
+    apply VarSet_For_all_Empty.
+    assumption.
 Qed.
 
 Lemma context_permutation : forall (c1 c2 : context) e t,
@@ -147,6 +309,12 @@ Proof.
     + rewrite Var.eqb_neq in Heqn.
       repeat (rewrite ContextFacts.add_neq_o; try trivial).
   - apply has_type_app with (t1:=t1); auto.
+  - (* Why does rewriting not work here but works a few steps later? *)
+    (* rewrite <- H2. *)
+    apply has_type_let with (t1:=t1); auto.
+    apply IHhas_type2.
+    rewrite H2.
+    apply ContextFacts.Equal_refl.
 Qed.
 
 Lemma context_add_add_eq : forall (c : context) x t1 t2,
@@ -182,153 +350,73 @@ Proof.
   - repeat (rewrite ContextFacts.add_neq_o; try trivial).
 Qed.
 
-Lemma context_weakening : forall (c : context) e t t' x,
-  has_type c e t ->
-  ~ VarSet.In x (free_vars e) ->
-  has_type (Context.add x t' c) e t.
-Proof.
-  intros c e t t' x H1.
-  generalize dependent x.
-  induction H1; intros ? H2.
-  - apply has_type_unit.
-  - apply has_type_var.
-    rewrite ContextFacts.add_neq_o.
-    + assumption.
-    + simpl in H2.
-      rewrite VarSetFacts.singleton_iff in H2.
-      congruence.
-  - apply has_type_abs.
-    destruct (Var.eqb x0 x) eqn:Heqn.
-    + rewrite Var.eqb_eq in Heqn; subst.
-      eauto using context_permutation, context_add_add_eq.
-    + rewrite Var.eqb_neq in Heqn.
-      eapply context_permutation.
-      * apply IHhas_type with (x0:=x0).
-        intros contra.
-        apply H2.
-        apply VarSetFacts.remove_2; auto.
-      * apply context_add_add_neq.
-        assumption.
-  - apply has_type_app with (t1:=t1);
-      try apply IHhas_type1;
-      try apply IHhas_type2;
-      intros H3; apply H2; simpl;
-      apply VarSet.union_spec;
-      auto.
-Qed.
-
-Lemma has_type_free_vars_in_context : forall c e t,
-  has_type c e t ->
-  VarSet.For_all (fun x => Context.mem x c = true) (free_vars e).
-Proof.
-  intros c e t H.
-  induction H; simpl.
-  - intros x contra.
-    apply VarSetFacts.empty_iff in contra.
-    inversion contra.
-  - intros y H2.
-    apply Context.mem_1.
-    apply ContextFacts.in_find_iff.
-    apply VarSet.singleton_spec in H2.
-    subst.
-    rewrite H.
-    discriminate.
-  - intros y H2.
-    unfold VarSet.For_all in *.
-    apply VarSet.remove_spec in H2 as [H2 H3].
-    specialize (IHhas_type y H2).
-    rewrite ContextFacts.add_neq_b in IHhas_type; auto.
-  - intros x H2.
-    apply VarSet.union_spec in H2 as [H2 | H2]; auto.
-Qed.
-
-Lemma has_type_empty_context_free_vars : forall e t,
-  has_type context_empty e t ->
-  VarSet.Empty (free_vars e).
-Proof.
-  intros e t H.
-  apply has_type_free_vars_in_context in H.
-  induction (free_vars e) using VarSetProps.set_induction.
-  - assumption.
-  - rename t0_1 into s.
-    rename t0_2 into s'.
-    apply VarSetProps.Add_Equal in H1.
-    unfold VarSet.For_all in *.
-    specialize (H x).
-    rewrite H1 in H.
-    specialize (H (VarSetFacts.add_1 s eq_refl)).
-    rewrite ContextFacts.empty_a in H.
-    discriminate.
-Qed.
-
 Lemma context_empty_weakening : forall (c c' : context) e t,
   has_type c e t ->
-  (forall x, VarSet.mem x (free_vars e) = true ->
-    Context.find x c = Context.find x c') ->
+  VarSet.For_all (fun x => Context.find x c = Context.find x c')
+    (free_vars e) ->
   has_type c' e t.
 Proof.
-  intros.
+  intros c c' e t H1.
   generalize dependent c'.
-  induction H; intros.
+  induction H1; intros c' H2.
   - apply has_type_unit.
   - apply has_type_var.
-    destruct (VarSet.mem x (free_vars (evar x))) eqn:Heqn.
-    + apply H0 in Heqn.
-      rewrite <- Heqn.
-      assumption.
-    + simpl in Heqn.
-      apply VarSetFacts.not_mem_iff in Heqn.
-      rewrite VarSetFacts.singleton_iff in Heqn.
-      congruence.
+    unfold VarSet.For_all in H2.
+    specialize (H2 _ (VarSetFacts.singleton_2 eq_refl)).
+    rewrite <- H2.
+    assumption.
   - apply has_type_abs.
     apply IHhas_type.
     intros y FREE_VAR.
+    simpl in H2.
     destruct (Var.eqb x y) eqn:Heqn.
-    + rewrite Var.eqb_eq in Heqn.
+    + apply Var.eqb_eq in Heqn.
       repeat (rewrite ContextFacts.add_eq_o; try assumption).
       reflexivity.
-    + rewrite Var.eqb_neq in Heqn.
+    + apply Var.eqb_neq in Heqn.
       repeat (rewrite ContextFacts.add_neq_o; try assumption).
-      apply H0.
-      simpl.
-      rewrite VarSetFacts.remove_neq_b; assumption.
+      auto using VarSetFacts.remove_2.
   - apply has_type_app with t1.
     + apply IHhas_type1.
       intros x FREE_VAR.
-      apply H1.
-      simpl.
-      rewrite VarSetFacts.union_b.
-      rewrite FREE_VAR.
-      reflexivity.
+      simpl in H2.
+      auto using VarSetFacts.union_2.
     + apply IHhas_type2.
       intros x FREE_VAR.
-      apply H1.
-      simpl.
-      rewrite VarSetFacts.union_b.
-      rewrite FREE_VAR.
-      apply orb_true_r.
+      simpl in H2.
+      auto using VarSetFacts.union_3.
+  - eapply has_type_let with t1.
+    + apply IHhas_type1.
+      intros y FREE_VAR.
+      simpl in H2.
+      auto using VarSetFacts.union_2.
+    + apply IHhas_type2.
+      intros y FREE_VAR.
+      destruct (Var.eqb x y) eqn:Heqn.
+      * apply Var.eqb_eq in Heqn.
+        repeat rewrite ContextFacts.add_eq_o; trivial.
+      * apply Var.eqb_neq in Heqn.
+        repeat rewrite ContextFacts.add_neq_o; trivial.
+        simpl in H2.
+        auto using VarSetFacts.union_3, VarSetFacts.remove_2.
 Qed.
 
-Lemma has_type_subst : forall e1 e2 c x t1 t2 ,
-  has_type (Context.add x t2 c) e1 t1 ->
-  has_type context_empty e2 t2 ->
-  has_type c (subst x e2 e1) t1.
+(* Lemma has_type_subst : forall e1 e2 c x t1 t2 ,
+  has_type c e1 t1 ->
+  Context.MapsTo x t2 c ->
+  VarSet.For_all (fun y => x <> y -> Context.find y c = Context.find y c')
+    (free_vars e1) ->
+  has_type c' e2 t2 ->
+  has_type c' (subst x e2 e1) t1.
 Proof.
-  induction e1; intros e2 c x t1 t2 H1 H2; inversion H1; subst.
+  induction e1; intros e2 c x t1 t2 H1 H2; inversion H1; clear H1; subst.
   - apply has_type_unit.
   - simpl.
     destruct (Var.eqb x v) eqn:Heqn.
     + rewrite Var.eqb_eq in Heqn.
       rewrite ContextFacts.add_eq_o in H3; try assumption.
       inversion H3; subst.
-      apply context_empty_weakening with context_empty.
-      * assumption.
-      * intros x FREE_VAR.
-        apply has_type_empty_context_free_vars in H2.
-        apply VarSetProps.empty_is_empty_1 in H2.
-        rewrite H2 in FREE_VAR.
-        rewrite VarSetFacts.empty_b in FREE_VAR.
-        inversion FREE_VAR.
+      assumption.
     + rewrite Var.eqb_neq in Heqn.
       rewrite ContextFacts.add_neq_o in H3; try assumption.
       apply has_type_var.
@@ -340,49 +428,184 @@ Proof.
       eauto using
         context_permutation, context_add_add_eq, ContextFacts.Equal_sym.
     + rewrite Var.eqb_neq in Heqn.
-      eauto using context_permutation, context_add_add_neq.
+      admit.
+(*       eauto using context_permutation, context_add_add_neq. *)
   - apply has_type_app with t0; eauto.
-Qed.
+  - simpl.
+    apply has_type_let with t0.
+    + eauto.
+    + destruct (x =? v) eqn:Heqn.
+      * rewrite Var.eqb_eq in Heqn; subst.
+        eauto using
+          context_permutation, context_add_add_eq, ContextFacts.Equal_sym.
+      * rewrite Var.eqb_neq in Heqn.
+        apply not_eq_sym in Heqn.
+        eapply IHe1_2.
+        { eauto using context_permutation, context_add_add_neq. }
+        { admit. }
+Admitted. *)
+
+Lemma has_type_subst : forall e1 e2 c x t1 t2 ,
+  has_type (Context.add x t2 c) e1 t1 ->
+  has_type c e2 t2 ->
+  VarSet.Empty (free_vars e2) ->
+  has_type c (subst x e2 e1) t1.
+Proof.
+  induction e1; intros e2 c x t1 t2 H1 H2 H3; inversion H1; clear H1; subst.
+  - apply has_type_unit.
+  - simpl.
+    destruct (Var.eqb x v) eqn:Heqn.
+    + rewrite Var.eqb_eq in Heqn.
+      rewrite ContextFacts.add_eq_o in H4; try assumption.
+      inversion H4; subst.
+      assumption.
+    + rewrite Var.eqb_neq in Heqn.
+      rewrite ContextFacts.add_neq_o in H4; try assumption.
+      apply has_type_var.
+      assumption.
+  - simpl.
+    apply has_type_abs.
+    destruct (Var.eqb x v) eqn:Heqn.
+    + rewrite Var.eqb_eq in Heqn; subst.
+      eauto using
+        context_permutation, context_add_add_eq, ContextFacts.Equal_sym.
+    + rewrite Var.eqb_neq in Heqn.
+      eapply IHe1.
+      * eauto using context_permutation, context_add_add_neq.
+      * admit.
+      * assumption.
+(*       eauto using context_permutation, context_add_add_neq. *)
+  - apply has_type_app with t0; eauto.
+  - simpl.
+    apply has_type_let with t0.
+    + eauto.
+    + destruct (x =? v) eqn:Heqn.
+      * rewrite Var.eqb_eq in Heqn; subst.
+        eauto using
+          context_permutation, context_add_add_eq, ContextFacts.Equal_sym.
+      * rewrite Var.eqb_neq in Heqn.
+        apply not_eq_sym in Heqn.
+        eapply IHe1_2.
+        { eauto using context_permutation, context_add_add_neq. }
+        { admit. }
+        { assumption. }
+Admitted.
+
+Lemma FOO1 : forall x t1 t2 (c : context),
+  Context.MapsTo x t1 c ->
+  Context.MapsTo x t2 c ->
+  t1 = t2.
+Proof. Admitted.
+
+Lemma FOO2 : forall x e1 e2 (c : heap),
+  Heap.MapsTo x e1 c ->
+  Heap.MapsTo x e2 c ->
+  e1 = e2.
+Proof. Admitted.
+
+Theorem preservation0 : forall c e1 e2 t h,
+  has_type c e1 t ->
+  VarSet.For_all (fun x => exists t e,
+    Context.MapsTo x t c /\ Heap.MapsTo x e h /\ has_type c e t) (free_vars e1) ->
+  eval h e1 e2 ->
+  has_type c e2 t.
+Proof.
+  intros c e1 e2 t h HAS_TYPE.
+  generalize dependent e2.
+  generalize dependent h.
+  induction HAS_TYPE; intros h e3 HH EVAL.
+  - inversion EVAL.
+  - inversion EVAL; clear EVAL; subst.
+    unfold VarSet.For_all in HH.
+    simpl in HH.
+    specialize (HH x (VarSetFacts.singleton_2 eq_refl))
+      as [ty [e [HH1 [HH2 HH3]]]].
+    apply Context.find_2 in H.
+    apply Heap.find_2 in H2.
+    erewrite FOO1 in *; try eassumption.
+    erewrite FOO2 with (e1:=e3) in *; eassumption.
+  - inversion EVAL.
+  - unfold VarSet.For_all in *.
+    inversion EVAL; clear EVAL; subst.
+    + apply has_type_app with t1; eauto using VarSetFacts.union_2.
+    + apply has_type_app with t1; eauto using VarSetFacts.union_3.
+    + inversion HAS_TYPE1; clear HAS_TYPE1; subst.
+      apply has_type_subst with t1.
+      * assumption.
+      * assumption.
+      * admit.
+  - unfold VarSet.For_all in *.
+    inversion EVAL; clear EVAL; subst.
+    + apply has_type_let with t1; eauto using VarSetFacts.union_2.
+    + apply has_type_subst with t1.
+      * assumption.
+      * assumption.
+      * admit.
+Admitted.
 
 Theorem preservation : forall e1 e2 t,
   has_type context_empty e1 t ->
-  eval e1 e2 ->
+  eval heap_empty e1 e2 ->
   has_type context_empty e2 t.
 Proof.
-  intros e1 e2 t HAS_TYPE.
-  generalize dependent e2.
-  remember context_empty as c.
-  induction HAS_TYPE; intros e3 EVAL.
+  intros e1.
+  induction e1; intros e2 ty HAS_TYPE EVAL.
   - inversion EVAL.
+  - inversion EVAL; clear EVAL; subst.
+    inversion H1.
   - inversion EVAL.
-  - inversion EVAL.
-  - inversion EVAL; subst.
-    + eauto using has_type_app.
-    + eauto using has_type_app.
-    + clear IHHAS_TYPE1.
-      clear IHHAS_TYPE2.
-      inversion HAS_TYPE1; subst.
-      eapply has_type_subst.
-      * eassumption.
-      * assumption.
+  - inversion HAS_TYPE; clear HAS_TYPE; subst.
+    inversion EVAL; clear EVAL; subst.
+    + apply has_type_app with t1.
+      * eauto.
+      * eauto.
+    + apply has_type_app with t1.
+      * eauto.
+      * eauto.
+    + inversion H2; clear H2; subst.
+      eauto using has_type_subst, has_type_empty_context_free_vars.
+  - inversion HAS_TYPE; clear HAS_TYPE; subst.
+    inversion EVAL; clear EVAL; subst.
+    + apply has_type_let with t1.
+      * eauto.
+      * eauto.
+    + eauto using has_type_subst, has_type_empty_context_free_vars.
 Qed.
+
+(* Theorem preservation : forall e1 e2 t,
+  has_type context_empty e1 t ->
+  eval heap_empty e1 e2 ->
+  has_type context_empty e2 t.
+Proof.
+  intros e1 e2 t HAS_TYPE EVAL.
+  eapply preservation0.
+  - eassumption.
+  - apply has_type_empty_context_free_vars in HAS_TYPE.
+    apply VarSetProps.empty_is_empty_1 in HAS_TYPE.
+    intros x FREE_VAR.
+    rewrite HAS_TYPE in FREE_VAR.
+    apply VarSetFacts.empty_iff in FREE_VAR.
+    inversion FREE_VAR.
+  - eassumption.
+Qed. *)
 
 Theorem preservation_eval_star : forall e1 e2 t,
   has_type context_empty e1 t ->
-  eval_star e1 e2 ->
+  eval_star heap_empty e1 e2 ->
   has_type context_empty e2 t.
 Proof.
   intros e1 e2 t H1 H2.
-  induction H2; eauto using preservation.
+  remember heap_empty as h.
+  induction H2; subst; eauto using preservation.
 Qed.
 
-Definition normal_form e := ~ exists e', eval e e'.
-Definition stuck e := normal_form e /\ ~ value e.
+Definition normal_form h e := ~ exists e', eval h e e'.
+Definition stuck h e := normal_form h e /\ ~ value e.
 
 Theorem soundness : forall e1 e2 t,
   has_type context_empty e1 t ->
-  eval_star e1 e2 ->
-  ~ stuck e2.
+  eval_star heap_empty e1 e2 ->
+  ~ stuck heap_empty e2.
 Proof.
   intros e1 e2 t H1 H2.
   unfold not, stuck, normal_form.
